src/kemedhoc/Impl.KEMEDHOC.Core.Msg2.fst
@@ -1,0 +1,66 @@
+module Impl.KEMEDHOC.Core.Msg2
+
+
+(*HACL Random lib*)
+open Lib.RandomBuffer.System
+
+module B = LowStar.Buffer
+module ST = FStar.HyperStack.ST
+module HS = FStar.HyperStack
+module S = FStar.Seq
+module Seq = Lib.Sequence
+
+module FBytes = FStar.Bytes
+
+(*Specification modules*)
+module Spec = Spec.KEMEDHOC.Core
+friend Spec.KEMEDHOC.Core
+
+module SpecCrypto = Spec.KEMEDHOC.CryptoPrimitives
+module SpecParser = Spec.KEMEDHOC.Parser
+
+module TypeEdhoc = TypeHelper.EDHOC
+module SpecEdhocSerd = Spec.EDHOC.Serialization
+
+
+(*------------------ Responder's side*)
+#push-options "--z3refresh --z3rlimit 60 --max_fuel 4 --max_ifuel 4"
+
+let responder_send_msg2 kcs rs hs msg1 msg2
+  = (**) let h0 = ST.get () in
+  responder_send_msg2_set_up kcs rs hs msg1 msg2;
+  let res = responder_construct_msg2 kcs rs hs msg2 in
+
+  (**) let h_final = ST.get () in
+  (**) assert(
+    lbufferOpt_is_Some h_final hs.k_xy /\ lbufferOpt_is_Some h_final hs.k_auth_I
+    /\ lbufferOpt_is_Some h_final hs.th2 /\ lbufferOpt_is_Some h_final hs.prk2e
+    /\ lbufferOpt_is_Some h_final hs.prk3e2m
+  );
+  (**) assume(
+    let rs_init = party_state_m_eval h0 rs in
+    let hs_init = handshake_state_m_eval h0 hs in
+    let msg1_init = message1_eval h0 msg1 in
+    let entr = B.deref h0 (entropy_p <: B.buffer (Ghost.erased HACLRandom.entropy)) in
+
+    let res_s = Spec.responder_send_msg2 kcs rs_init hs_init msg1_init entr in
+
+    let hs_s_final = handshake_state_m_eval h_final hs in
+    let msg2_s_final = message2_eval h_final msg2 in
+
+    match res_s with
+      | Fail e -> res == error_to_c_response e
+      | Res (m2_s, hs_s) -> (
+        res == TypeEdhoc.CSuccess
+        /\ Spec.hs_equal hs_s_final hs_s
+        /\ SpecParser.message2_equal msg2_s_final m2_s
+      )
+    
+    );
+    res
+
+#pop-options
+
+(*------------------ Initiator's side*)
+let initiator_process_msg2 kcs is hs msg2 p2
+  = TypeEdhoc.CSuccess
