src/kemedhoc/Impl.KEMEDHOC.Core.Msg2.fsti
@@ -1,0 +1,144 @@
+module Impl.KEMEDHOC.Core.Msg2
+
+(*LowStar related modules*)
+open Lib.ByteBuffer
+open Lib.IntTypes
+open Lib.Buffer
+
+(*HACL Random lib*)
+open Lib.RandomBuffer.System
+module HACLRandom = Lib.RandomSequence
+
+module B = LowStar.Buffer
+module ST = FStar.HyperStack.ST
+module HS = FStar.HyperStack
+module S = FStar.Seq
+module Seq = Lib.Sequence
+
+(*Specification modules*)
+module Spec = Spec.KEMEDHOC.Core
+
+module SpecCrypto = Spec.KEMEDHOC.CryptoPrimitives
+module SpecParser = Spec.KEMEDHOC.Parser
+module SpecTH = Spec.KEMEDHOC.TranscriptHash
+module SpecKS = Spec.KEMEDHOC.KeySchedule
+
+module SpecEdhocSerd = Spec.EDHOC.Serialization
+
+module TypeEdhoc = TypeHelper.EDHOC
+
+(*EDHOC utilities*)
+open Impl.EDHOC.Utilities
+
+(*KEMEDHOC utilities*)
+open Impl.KEMEDHOC.Types
+open Impl.KEMEDHOC.CryptoPrimitives
+open Impl.KEMEDHOC.KeySchedule
+open Impl.KEMEDHOC.Parser
+open Impl.KEMEDHOC.Ciphertext
+open Impl.KEMEDHOC.TranscriptHash
+open Impl.KEMEDHOC.Core
+open Spec.KEMEDHOC.Base.Definitions
+
+open Impl.KEMEDHOC.Core.Msg2.Aux
+
+(*------------------ Responder's side*)
+val responder_send_msg2:
+  kcs: supportedKemCipherSuite
+  -> rs: party_state_m kcs
+  -> hs: handshake_state_m kcs
+  -> msg1: message1 kcs
+  -> msg2: message2 kcs
+  -> ST.Stack c_response
+  (requires fun h0 ->
+    is_valid_handshake_state_m h0 hs
+    /\ is_valid_party_state_m h0 rs
+    /\ is_valid_message1 h0 msg1 /\ is_legit_message1 h0 msg1
+    /\ is_valid_message2 h0 msg2
+    /\ live h0 entropy_p /\ live h0 kem_state
+
+    /\ (let hs_init = handshake_state_m_eval h0 hs in
+      Spec.is_valid_handshake_state_init hs_init
+    )
+
+    // Disjointness
+    /\ handshake_state_m_disjoint_to_party_state hs rs
+    /\ handshake_state_m_disjoint_to_msg1 hs msg1
+    /\ handshake_state_m_disjoint_to_msg2 hs msg2
+    /\ handshake_state_m_disjoint_to_lbuffer hs entropy_p
+    /\ handshake_state_m_disjoint_to_lbuffer hs kem_state
+    /\ party_state_disjoint_to_msg1 rs msg1
+    /\ party_state_disjoint_to_msg2 rs msg2
+    /\ party_state_disjoint_to_lbuffer rs entropy_p
+    /\ party_state_disjoint_to_lbuffer rs kem_state
+    /\ message2_disjoint_to_msg1 msg2 msg1
+    /\ message2_disjoint_to_lbuffer msg2 entropy_p
+    /\ message2_disjoint_to_lbuffer msg2 kem_state
+    /\ message1_disjoint_to_lbuffer msg1 entropy_p
+    /\ message1_disjoint_to_lbuffer msg1 kem_state
+    /\ disjoint kem_state entropy_p
+  )
+  (ensures fun h0 res h1 ->
+    
+    let modified_locs = loc kem_state |+| loc entropy_p
+              |+| lbufferOpt_loc hs.k_xy |+| loc msg2.ct_y
+              |+| lbufferOpt_loc hs.k_auth_I |+| loc msg2.ct_auth_I
+              |+| lbufferOpt_loc hs.th2
+              |+| lbufferOpt_loc hs.prk2e |+| lbufferOpt_loc hs.prk3e2m in 
+
+    (match res with
+      | TypeEdhoc.CUnsupportedAlgorithmOrInvalidConfig -> modifies modified_locs h0 h1
+      | TypeEdhoc.CSuccess -> modifies (modified_locs |+| loc msg2.c2) h0 h1
+      | _ -> False)
+    /\ (is_valid_handshake_state_m h1 hs
+      /\ Spec.is_valid_handshake_state_after_msg2 (handshake_state_m_eval h1 hs)
+      /\ is_valid_party_state_m h1 rs
+      /\ is_valid_message2 h1 msg2
+    )
+    /\ (
+      let rs_init = party_state_m_eval h0 rs in
+      let hs_init = handshake_state_m_eval h0 hs in
+      let msg1_init = message1_eval h0 msg1 in
+      let entr = B.deref h0 (entropy_p <: B.buffer (Ghost.erased HACLRandom.entropy)) in
+
+      let res_s = Spec.responder_send_msg2 kcs rs_init hs_init msg1_init entr in
+
+      let hs_s_final = handshake_state_m_eval h1 hs in
+      let msg2_s_final = message2_eval h1 msg2 in
+
+      match res_s with
+        | Fail e -> res == error_to_c_response e
+        | Res (m2_s, hs_s) -> (
+          res == TypeEdhoc.CSuccess
+          /\ Spec.hs_equal hs_s_final hs_s
+          /\ SpecParser.message2_equal msg2_s_final m2_s
+        )
+    )
+  )
+
+
+(*-------------------- Initiator's side*)
+val initiator_process_msg2:
+  kcs: supportedKemCipherSuite
+  -> is: party_state_m kcs
+  -> hs: handshake_state_m kcs
+  -> msg2: message2 kcs
+  -> p2: plaintext2 kcs
+  -> ST.Stack c_response
+  (requires fun h0 ->
+    is_valid_handshake_state_m h0 hs
+    /\ is_valid_party_state_m h0 is
+    /\ is_valid_message2 h0 msg2
+    /\ is_valid_plaintext2 h0 p2
+
+    // Disjointness
+    /\ handshake_state_m_disjoint_to_party_state hs is
+    /\ handshake_state_m_disjoint_to_msg2 hs msg2
+    /\ handshake_state_m_disjoint_to_p2 hs p2
+    /\ party_state_disjoint_to_msg2 is msg2
+    /\ party_state_disjoint_to_p2 is p2
+    /\ message2_disjoint_to_p2 msg2 p2
+  )
+  (ensures fun h0 res h1 ->
+    True
+  )
